progs/VSUpile/verif_onepile.v
@@ -10,24 +10,81 @@ Instance OnePileCompSpecs : compspecs. make_compspecs prog. Defined.
 Section Onepile_VSU.
 Variable M: MallocFreeAPD.
 Variable PILE: PileAPD. (*onepile is parametric in a pile predicate structure*)
-
-Definition one_pile (gv: globals) (sigma: option (list Z)) : mpred :=
+(*
+Definition one_pile' (sigma: option (list Z)) (gv: globals) : mpred :=
  match sigma with
- | None => data_at_ Ews (tptr tpile) (gv _the_pile)
+ | None =>  data_at_ Ews (tptr tpile) (*memory_block Ews 4*) (gv _the_pile)
+            (*data_at Ews (tptr tpile) nullval (gv _the_pile)*)
  | Some il => EX p:val, data_at Ews (tptr tpile) p (gv _the_pile) *
-                               pilerep PILE il p * pile_freeable PILE p
+                        pilerep PILE il p * pile_freeable PILE p
+ end.
+Definition one_pile (sigma: option (list Z)) (gv: globals) : mpred := 
+ !!(headptr (gv _the_pile)) && one_pile' sigma gv.
+*)
+Definition one_pile (sigma: option (list Z)) (gv: globals) : mpred := 
+(* !!(headptr (gv _the_pile)) &&*)
+match sigma with
+ | None =>  data_at_ Ews (tptr tpile) (*memory_block Ews 4*) (gv _the_pile)
+            (*data_at Ews (tptr tpile) nullval (gv _the_pile)*)
+ | Some il => EX p:val, data_at Ews (tptr tpile) p (gv _the_pile) *
+                        pilerep PILE il p * pile_freeable PILE p
  end.
 
-Lemma make_onepile: forall gv, 
+Lemma make_onepile: forall gv, (*headptr (gv _the_pile) ->*)
   data_at_ Ews (tptr (Tstruct onepile._pile noattr)) (gv onepile._the_pile)
-   |-- one_pile gv None.
+   |-- one_pile None gv.
 Proof.
 intros.
-unfold onepile.
-cancel.
+unfold onepile, one_pile. entailer!.
 Qed.
+(*
+Lemma make_onepile: forall gv, headptr (gv _the_pile) ->
+  data_at Ews (tptr (Tstruct onepile._pile noattr)) nullval (gv onepile._the_pile)
+   = one_pile None gv.
+Proof.
+intros.
+unfold one_pile. simpl. apply pred_ext.
++ entailer!.
++ entailer!.
+Qed.*)
+(*
+  Lemma MyInitData gv (H: headptr (gv _the_pile)):
+        initialize.gv_globvar2pred gv (_the_pile, v_the_pile) gv 
+        = data_at Ews (tptr tpile) nullval (gv _the_pile).
+  Proof. unfold initialize.gv_globvar2pred. simpl.
+         unfold initialize.gv_lift2, initialize.gv_lift0; simpl.
+         rewrite predicates_sl.sepcon_emp. forget (gv _the_pile) as p.
+         erewrite <- (mapsto_data_at'' Ews (tptr tpile)); trivial. clear - H.
+         unfold tpile, tptr. rewrite mapsto_size_t_tptr_nullval.
+         reflexivity.
+  Qed.
+  Lemma onepile_Init gv: InitGPred (Vardefs prog) gv |-- one_pile None gv.
+  Proof. unfold InitGPred, one_pile. simpl; Intros. rewrite sepcon_emp, MyInitData; trivial; entailer!. Qed.
+*)
+  Lemma onepile_Init_aux gv: headptr (gv _the_pile) ->
+    initialize.gv_globvar2pred gv (_the_pile, v_the_pile) gv
+    |-- data_at_ Ews (tptr (Tstruct _pile noattr)) (gv _the_pile).
+  Proof. intros.
+    unfold initialize.gv_globvar2pred. simpl.
+         unfold initialize.gv_lift2, initialize.gv_lift0; simpl.
+         rewrite predicates_sl.sepcon_emp.
+    destruct H as [b Hb]; rewrite Hb in *.
+    eapply derives_trans. 
+    + apply mapsto_zeros_memory_block. apply writable_readable. apply writable_Ews.
+    + rewrite <- memory_block_data_at_; simpl; trivial.
+      apply headptr_field_compatible; trivial. exists b; trivial. cbv; trivial. simpl; rep_omega.
+      econstructor. reflexivity. apply Z.divide_0_r.
+  Qed.
 
-Definition ONEPILE: OnePileAPD := Build_OnePileAPD one_pile OnePileCompSpecs make_onepile.
+  Lemma onepile_Init_aux2 gv: headptr (gv _the_pile) ->
+    initialize.gv_globvar2pred gv (_the_pile, v_the_pile) gv
+    |--  one_pile None gv.
+  Proof. intros. sep_apply onepile_Init_aux. apply make_onepile; trivial. Qed.
+
+  Lemma onepile_Init gv: InitGPred (Vardefs prog) gv |-- one_pile None gv.
+  Proof. unfold InitGPred. simpl; Intros. sep_apply onepile_Init_aux2; trivial. simpl; trivial. Qed.
+
+Definition ONEPILE: OnePileAPD := Build_OnePileAPD one_pile(* OnePileCompSpecs make_onepile*) (*_  onepile_Init*).
 
   Definition Onepile_ASI: funspecs := OnepileASI M ONEPILE.
 
@@ -50,9 +107,13 @@ Proof.
 start_function.
 forward_call gv.
 Intros p.
-simpl onepile. unfold one_pile.
+simpl onepile; unfold one_pile(*; simpl one_pile'*); Intros.
+(*specialize (memory_block_data_at_ Ews (tptr tpile)); simpl; intros X.
+rewrite X; clear X.
+2:{ red; simpl. destruct HP_the_pile. rewrite H in *. repeat split; trivial.
+    eapply align_compatible_rec_by_value. cbv; reflexivity. apply Z.divide_0_r. }*)
 forward.
-simpl onepile. unfold one_pile.
+simpl onepile; unfold one_pile(*; simpl one_pile'*).
 Exists p.
 entailer!.
 Qed.
@@ -60,12 +121,12 @@ Qed.
 Lemma body_Onepile_add: semax_body OnepileVprog OnepileGprog f_Onepile_add (Onepile_add_spec M ONEPILE).
 Proof.
 start_function.
-simpl onepile. unfold one_pile.
+simpl onepile; unfold one_pile(*; simpl one_pile'*); Intros.
 Intros p.
 forward.
 forward_call (p,n,sigma,gv).
 forward.
-simpl onepile. unfold one_pile.
+simpl onepile; unfold one_pile(*; simpl one_pile'*).
 Exists p.
 entailer!.
 Qed.
@@ -73,25 +134,42 @@ Qed.
 Lemma body_Onepile_count: semax_body OnepileVprog OnepileGprog f_Onepile_count (Onepile_count_spec ONEPILE).
 Proof.
 start_function.
-simpl onepile. unfold one_pile in *.
+simpl onepile; unfold one_pile(*; simpl one_pile'*); Intros.
 Intros p.
 forward.
 forward_call (p,sigma).
 forward.
+simpl onepile; unfold one_pile(*; simpl one_pile'*).
 Exists p.
 entailer!.
 Qed.
+(*hold but dead
+Lemma GG: globvar2pred = initialize.globvar2pred. reflexivity. Qed.
+
+  Lemma globEntailsInitPred g:
+        globvar2pred (globals_of_env (Clight_seplog.mkEnv g [] [])) (onepile._the_pile, onepile.v_the_pile)
+                    (Clight_seplog.mkEnv g [] [])
+        |-- one_pile None (globals_of_env (Clight_seplog.mkEnv g [] [])).
+  Proof. unfold one_pile, one_pile'. rewrite GG, initialize.globvar2pred_char_gv. simpl. unfold initialize.gv_globvar2pred. simpl.
+         unfold initialize.gv_lift2, initialize.gv_lift0; simpl.
+         rewrite predicates_sl.sepcon_emp. rewrite mapsto_isptr; Intros. apply global_is_headptr in H.
+         erewrite <- (mapsto_data_at'' Ews (tptr tpile)); trivial. entailer!. clear - H.
+         unfold tpile, tptr. rewrite mapsto_size_t_tptr_nullval. apply derives_refl.
+  Qed.*)
 
   Definition OnepileComponent: @Component NullExtension.Espec OnepileVprog _ 
-      nil onepile_imported_specs prog Onepile_ASI onepile_internal_specs.
-  Proof. 
+      nil onepile_imported_specs prog Onepile_ASI (one_pile None) onepile_internal_specs.
+  Proof.
     mkComponent. 
     + solve_SF_internal body_Onepile_init.
     + solve_SF_internal body_Onepile_add.
     + solve_SF_internal body_Onepile_count.
+    + intros. (* unfold InitGPred, one_pile; simpl. entailer!.
+      rewrite MyInitData; trivial; cancel.*) 
+      sep_apply (onepile_Init gv); simpl; cancel.
   Qed.
 
 Definition OnepileVSU: @VSU NullExtension.Espec OnepileVprog _ 
-      nil onepile_imported_specs prog Onepile_ASI.
+      nil onepile_imported_specs prog Onepile_ASI (one_pile None).
   Proof. eexists; apply OnepileComponent. Qed.
 End Onepile_VSU.
